Semantics/Imp/Untyped/Natural.lean
@@ -3,78 +3,78 @@ import Semantics.Imp.Untyped.Bexp
 namespace Com
 namespace Natural
 
-inductive Step: Com × State → State → Prop
+inductive Step: Com → State → State → Prop
   | skip:
-    Step (skip, s) s
+    Step skip s s
 
   | ass:
-    Step (ass x a, s) (s⟪x ≔ a.reduce s⟫)
+    Step (ass x a) s (s⟪x ≔ a⇓s⟫)
 
   | cat t
-    (hc: Step (c, s) t) (hd: Step (d, t) u):
-    Step (c;;d, s) u
+    (hc: Step c s t) (hd: Step d t u):
+    Step (c;;d) s u
 
   | cond₁ {b: Bexp}
-    (hb: b.reduce s = true) (hc: Step (c, s) t):
-    Step (cond b c d, s) t
+    (hb: b⇓s = true) (hc: Step c s t):
+    Step (cond b c d) s t
 
   | cond₂ {b: Bexp}
-    (hb: b.reduce s = false) (hd: Step (d, s) t):
-    Step (cond b c d, s) t
+    (hb: b⇓s = false) (hd: Step d s t):
+    Step (cond b c d) s t
 
   | loop₁ {b: Bexp} u
-    (hb: b.reduce s = true) (hc: Step (c, s) u) (hw: Step (loop b c, u) t):
-    Step (loop b c, s) t
+    (hb: b⇓s = true) (hc: Step c s u) (hw: Step (loop b c) u t):
+    Step (loop b c) s t
 
   | loop₂ {b: Bexp}
-    (hb: b.reduce s = false):
-    Step (loop b c, s) s
+    (hb: b⇓s = false):
+    Step (loop b c) s s
 
-infix:110 " ⟹ " => Step
+notation s " ⊢ " c " ⟹ " t => Step c s t
 
-theorem demo₁: (⦃x = 5⦄, ⟪⟫) ⟹ ⟪⟫⟪"x"≔5⟫ := Step.ass
+theorem demo₁: ⟪⟫ ⊢ ⦃x = 5⦄ ⟹ ⟪"x" ≔ 5⟫ := Step.ass
 
 theorem demo₂:
-  (⦃x = 2; if x <= 1 {y = 3} else {z = 4}⦄, ⟪⟫) ⟹
-  (⟪⟫⟪"x"≔2⟫⟪"z"≔4⟫) := Step.cat _ Step.ass $ Step.cond₂ rfl Step.ass
+  ⟪⟫ ⊢ ⦃x = 2; if x <= 1 {y = 3} else {z = 4}⦄ ⟹ ⟪"x" ≔ 2⟫⟪"z" ≔ 4⟫ :=
+    Step.cat _ Step.ass $ Step.cond₂ rfl Step.ass
 
 /-
 ## Rewriting rules
 -/
 
-theorem skip_iff: (skip, s) ⟹ t ↔ s = t := by
+theorem skip_iff: (s ⊢ skip ⟹ t) ↔ s = t := by
   apply Iff.intro <;> intro h
   . cases h; rfl
   . exact h ▸ Step.skip
 
-theorem cat_iff: (c;;d, s) ⟹ t ↔ ∃ w, (c, s) ⟹ w ∧ (d, w) ⟹ t := by
+theorem cat_iff: (s ⊢ c;;d ⟹ t) ↔ ∃ w, (s ⊢ c ⟹ w) ∧ (w ⊢ d ⟹ t) := by
   apply Iff.intro <;> intro h
   . cases h with | cat t h₁ h₂ =>
       exact ⟨t, ⟨h₁, h₂⟩⟩
   . cases h with | intro w h =>
       exact Step.cat w h.1 h.2
 
-theorem cond_iff: (cond b c d, s) ⟹ t ↔ bif b.reduce s then (c, s) ⟹ t else (d, s) ⟹ t := by
+theorem cond_iff: (s ⊢ cond b c d ⟹ t) ↔ bif b⇓s then (s ⊢ c ⟹ t) else (s ⊢ d ⟹ t) := by
   constructor <;> intro h
   . cases h with
     | cond₁ hb hc => exact hb ▸ hc
     | cond₂ hb hc => exact hb ▸ hc
-  . cases hb: b.reduce s with
-    | true => exact Step.cond₁ hb $ (cond_true ((c, s) ⟹ t) _) ▸ hb ▸ h
-    | false => exact Step.cond₂ hb $ (cond_false _ ((d, s) ⟹ t)) ▸ hb ▸ h
+  . cases hb: b⇓s with
+    | true => exact Step.cond₁ hb $ (cond_true (s ⊢ c ⟹ t) _) ▸ hb ▸ h
+    | false => exact Step.cond₂ hb $ (cond_false _ (s ⊢ d ⟹ t)) ▸ hb ▸ h
 
-theorem cond_iff': (cond b c d, s) ⟹ t ↔ (bif b.reduce s then c else d, s) ⟹ t := by
-  rw [cond_iff]; cases b.reduce s <;> simp
+theorem cond_iff': (s ⊢ cond b c d ⟹ t) ↔ (s ⊢ bif b⇓s then c else d ⟹ t) := by
+  rw [cond_iff]; cases b⇓s <;> simp
 
-theorem loop_iff: (loop b c, s) ⟹ t ↔
-  (bif b.reduce s then ∃ w, (c, s) ⟹ w ∧ (loop b c, w) ⟹ t else s = t) := by
+theorem loop_iff: (s ⊢ loop b c ⟹ t) ↔
+  (bif b⇓s then ∃ w, (s ⊢ c ⟹ w) ∧ (w ⊢ loop b c ⟹ t) else s = t) := by
   apply Iff.intro <;> intro h
   . cases h with
     | loop₁ t hb hc hw =>
       exact hb ▸ ⟨t, ⟨hc, hw⟩⟩
     | loop₂ hb =>
       exact hb ▸ rfl
-  . cases hb: b.reduce s with
+  . cases hb: b⇓s with
     | true =>
       rw [hb] at h
       cases h with | intro w h =>
@@ -87,7 +87,7 @@ theorem loop_iff: (loop b c, s) ⟹ t ↔
 -/
 
 instance equiv: Setoid Com where
-  r c d := ∀ s t, (c, s) ⟹ t ↔ (d, s) ⟹ t
+  r c d := ∀ s t, (s ⊢ c ⟹ t) ↔ (s ⊢ d ⟹ t)
   iseqv := {
     refl := λ _ _ _ ↦ Iff.refl _
     symm := (Iff.symm $ · · ·)
@@ -128,19 +128,19 @@ theorem loop_unfold:
     | loop₂ hb => exact hb ▸ Step.skip
   . rw [loop_iff]
     rw [cond_iff] at h
-    cases hb: b.reduce s <;> rw [hb] at h
+    cases hb: b⇓s <;> rw [hb] at h
     . exact skip_iff.mp h
     . exact cat_iff.mp h
 
 /-
-## No normalization
+## No termination
 -/
 
 theorem loop_tt (h: b ≈ Bexp.tt):
-  ¬((loop b c, s) ⟹ t) := by
+  ¬(s ⊢ loop b c ⟹ t) := by
   intro h₁
-  generalize h₂: (loop b c, s) = ww at h₁
-  induction h₁ generalizing s with
+  generalize h₂: loop b c = ww at h₁
+  induction h₁ with
   | loop₁ _ _ _ _ _ ih₂ => cases h₂; apply ih₂; rfl
   | loop₂ hb => cases h₂; rw [h] at hb; contradiction
   | _ => cases h₂
@@ -149,7 +149,7 @@ theorem loop_tt (h: b ≈ Bexp.tt):
 ## Determinism
 -/
 
-theorem determinist {x: Com × State} (h₁: x ⟹ s) (h₂: x ⟹ t): s = t :=
+theorem determinist {c: Com} (h₁: w ⊢ c ⟹ s) (h₂: w ⊢ c ⟹ t): s = t :=
   by induction h₁ generalizing t with
   | cat _ _ _ ih₁ ih₂ => cases h₂ with
     | cat _ hc hd => exact ih₂ (ih₁ hc ▸ hd)
