Semantics/Imp/Untyped/Equivalence.lean
@@ -4,7 +4,7 @@ import Semantics.Imp.Untyped.Denote
 
 namespace Com
 
-theorem Structural.from_natural {x: Com × State} (h: x ⟹ s): x ⇒* (skip, s) := by
+theorem Structural.from_natural {c: Com} (h: w ⊢ c ⟹ s): (c, w) ⇒* (skip, s) := by
   induction h with
   | skip => exact Relation.ReflTransGen.refl
   | ass => exact Relation.ReflTransGen.single Step.ass
@@ -16,7 +16,7 @@ theorem Structural.from_natural {x: Com × State} (h: x ⟹ s): x ⇒* (skip, s)
   | loop₂ hb =>
     exact Relation.ReflTransGen.head Step.loop $ hb ▸ Relation.ReflTransGen.refl
 
-lemma Natural.from_structural_step (h₁: x ⇒ y) (h₂: y ⟹ s): x ⟹ s := by
+lemma Natural.from_structural_step (h₁: x ⇒ y) (h₂: y.2 ⊢ y.1  ⟹ s): x.2 ⊢ x.1 ⟹ s := by
   induction h₁ generalizing s with
   | ass => exact (skip_iff.mp h₂) ▸ Step.ass
   | cat₁ => exact Step.cat _ Step.skip h₂
@@ -26,14 +26,14 @@ lemma Natural.from_structural_step (h₁: x ⇒ y) (h₂: y ⟹ s): x ⟹ s := b
   | cond => rw [cond_iff']; exact h₂
   | loop => rw [loop_unfold, cond_iff']; exact h₂
 
-theorem Natural.from_structural (h: x ⇒* (skip, t)): x ⟹ t := by
+theorem Natural.from_structural (h: x ⇒* (skip, t)): x.2 ⊢ x.1 ⟹ t := by
   induction h using Relation.ReflTransGen.head_induction_on with
   | refl => exact Step.skip
   | head h _ ht => exact from_structural_step h ht
 
-theorem structural_iff_natural: x ⇒* (skip, t) ↔ x ⟹ t := ⟨Natural.from_structural, Structural.from_natural⟩
+theorem structural_iff_natural: (c, s) ⇒* (skip, t) ↔ (s ⊢ c ⟹ t) := ⟨Natural.from_structural, Structural.from_natural⟩
 
-theorem denote.from_natural {x: Com × State} (h: x ⟹ t): (x.2, t) ∈ ⟦x.1⟧ := by
+theorem denote.from_natural {c: Com} (h: s ⊢ c ⟹ t): (s, t) ∈ ⟦c⟧ := by
   induction h with
   | skip => exact SRel.mem_id.mpr rfl
   | ass  => exact SRel.mem_id.mpr rfl
@@ -43,7 +43,7 @@ theorem denote.from_natural {x: Com × State} (h: x ⟹ t): (x.2, t) ∈ ⟦x.1�
   | loop₁ t hb _ _ ih₁ ih₂ => exact loop_unfold ▸ Or.inl ⟨⟨t, ⟨ih₁, ih₂⟩⟩, hb⟩
   | loop₂ hb => exact loop_unfold ▸ Or.inr ⟨rfl, hb⟩
 
-theorem Natural.from_denote (h: (s, t) ∈ ⟦c⟧): (c, s) ⟹ t := by
+theorem Natural.from_denote (h: (s, t) ∈ ⟦c⟧): s ⊢ c ⟹ t := by
   revert h
   induction c generalizing s t with
   | skip => intro h; cases h; exact Step.skip
@@ -62,7 +62,7 @@ theorem Natural.from_denote (h: (s, t) ∈ ⟦c⟧): (c, s) ⟹ t := by
       cases h with | intro h hb =>
         exact Step.cond₂ hb (ih₂ h)
   | loop b c ih =>
-    suffices ⟦loop b c⟧ ⊆ {s | (loop b c, s.1) ⟹ s.2} by apply this
+    suffices ⟦loop b c⟧ ⊆ {s | s.1 ⊢ loop b c ⟹ s.2} by apply this
     apply OrderHom.lfp_le
     intro ss h
     cases ss with | mk =>
@@ -76,6 +76,6 @@ theorem Natural.from_denote (h: (s, t) ∈ ⟦c⟧): (c, s) ⟹ t := by
           simp at hq
           exact hq ▸ Step.loop₂ hb
 
-theorem natural_iff_denote: (s, t) ∈ ⟦c⟧ ↔ (c, s) ⟹ t := ⟨Natural.from_denote, denote.from_natural⟩
+theorem natural_iff_denote: (s, t) ∈ ⟦c⟧ ↔ (s ⊢ c ⟹ t) := ⟨Natural.from_denote, denote.from_natural⟩
 
 end Com
