Semantics/Imp/Untyped/Lang.lean
@@ -7,13 +7,14 @@ def State := String → Val
 def State.nil: State := λ _ ↦ 0
 
 notation "⟪⟫" => State.nil
-notation s "⟪" x "≔" e "⟫" => Function.update s x e
+notation s "⟪" x " ≔ " e "⟫" => Function.update s x e
+notation "⟪" x " ≔ " e "⟫" => ⟪⟫⟪x ≔ e⟫
 
 #reduce ⟪⟫ "x"
-#reduce (⟪⟫⟪"x" ≔ 3⟫⟪"x" ≔ 4⟫) "x"
-#reduce (⟪⟫⟪"x" ≔ 3⟫⟪"x" ≔ 4⟫⟪"x" ≔ 7⟫) "x"
+#reduce (⟪"x" ≔ 3⟫⟪"x" ≔ 4⟫) "x"
+#reduce (⟪"x" ≔ 3⟫⟪"x" ≔ 4⟫⟪"x" ≔ 7⟫) "x"
 
-theorem State.demo₁: (⟪⟫⟪"x"≔3⟫) = (⟪⟫⟪"x"≔4⟫⟪"x"≔3⟫) := by simp
+theorem State.demo₁: ⟪"x" ≔ 3⟫ = ⟪"x" ≔ 4⟫⟪"x" ≔ 3⟫ := by simp
 
 inductive Aexp where
   | val : Val → Aexp
