Semantics/Stlc/Typing.lean
@@ -1,4 +1,4 @@
-import Semantics.Stlc.Natural
+import Semantics.Stlc.Rewrite
 import Mathlib.Logic.Function.Basic
 
 def Context := String → Option Ty
@@ -12,9 +12,9 @@ inductive HasTy: Context → Term → Ty → Prop where
   | app (h₁: HasTy Γ t₁ (Ty.Arrow T₂ T₁)) (h₂: HasTy Γ t₂ T₂):
     HasTy Γ (Term.app t₁ t₂) T₁
   | true:
-    HasTy Γ (Term.true) Ty.Bool
+    HasTy Γ Term.tt Ty.Bool
   | false:
-    HasTy Γ (Term.false) Ty.Bool
+    HasTy Γ Term.ff Ty.Bool
   | cond (h₁: HasTy Γ b Ty.Bool) (h₂: HasTy Γ t₁ T₁) (h₃: HasTy Γ t₂ T₁):
     HasTy Γ (Term.cond b t₁ t₂) T₁
 
@@ -28,11 +28,48 @@ theorem typing_example_1:
 -/
 
 theorem canonical_form_bool
-  (h₁: empty_ctx ⊢ t : Ty.Bool) (h₂: Term.Value t):
-  (t = Term.true) ∨ (t = Term.false) :=
+  (h₁: empty_ctx ⊢ t : Ty.Bool) (h₂: value t):
+  (t = Term.tt) ∨ (t = Term.ff) :=
   by cases h₁ <;> cases h₂ <;> simp
 
 theorem canonical_form_fun
-  (h₁: empty_ctx ⊢ t : (Ty.Arrow T₁ T₂)) (h₂: Term.Value t):
+  (h₁: empty_ctx ⊢ t : (Ty.Arrow T₁ T₂)) (h₂: value t):
   ∃x u, t = (Term.abs x T₁ u) :=
   by cases h₁ <;> cases h₂; simp
+
+/-
+## Progress
+-/
+
+theorem progress (h: empty_ctx ⊢ t : T):
+  value t ∨ ∃t', t ⇒ t' := by
+  {
+    generalize he: empty_ctx = Γ at h
+    induction h <;> cases he
+    . rename_i h; cases h
+    . exact Or.inl rfl
+    . simp at *
+      rename_i t₁ _ _ t₂ h₁ h₂ ih₁ ih₂
+      apply Or.inr
+      cases ih₁ with
+      | inl h =>
+        cases ih₂ with
+        | inl hh =>
+          have hc := canonical_form_fun h₁ h
+          cases hc with
+          | intro x hc =>
+            cases hc with
+            | intro w hc =>
+              rw [hc]
+              exists [x≔t₂]w
+              exact step.appabs hh
+        | inr h => {
+          sorry
+        }
+      | inr h =>
+        cases h with
+        | intro w h =>
+          exists (Term.app w t₂)
+          apply step.app₁ h
+
+  }
